utils/Library_extra/Monoid_extra.thy
@@ -261,14 +261,11 @@ text \<open> In this theory we present a variant of the trace algebra where inst
 
 subsection \<open> Unary fzero \<close>
 
-text \<open> We call the unitary function fzero @{term f\<^sub>0}, that is, a functional zero
+text \<open> We call the unary function fzero @{term f\<^sub>0}, that is, a "functional zero"
        when compared to the monoid-based trace algebra. \<close>
   
 class fzero = 
   fixes fzero :: "'a \<Rightarrow> 'a" ("f0'(_')")
-
-class fzero_idem = fzero +
-  assumes fzero_idem[simp]: "f0(f0(a)) = f0(a)"    
 
 text \<open> The monoid-based trace algebra can be obtained by fixing @{term f\<^sub>0} as 0.
        We explore this in the trace algebra hierarchy theory file \<close>
@@ -287,55 +284,37 @@ subsection \<open> Unary fzero semigroup \<close>
 
 text \<open> The class of semigroups with a unary function is then defined. \<close>
 
+(* USTA1 *)
 class semigroup_add_fzero = semigroup_add + fzero
     
 text \<open> We then define mirror properties of a monoid, but instead we
        require the zero property on fzero, rather than 0. \<close>
     
-class fzero_add_zero = fzero_idem + semigroup_add_fzero +
-  assumes add_fzero_left[simp]: "f0(a) + a = a"
+(* USTA2 *)
+class fzero_right_ident = fzero + plus +
   assumes add_fzero_right[simp]: "a + f0(a) = a"
-
-class fzero_add_zero_any = fzero_add_zero +
-    assumes add_fzero_any_left[simp]: "f0(b) + a = a"
-
-instance fzero_add_zero_any \<subseteq> fzero_add_zero
-  by (intro_classes)
-      
+    
+(* USTA3 *)
+class add_left_cancel = plus +
+  assumes add_left_imp_eq: "a + b = a + c \<Longrightarrow> b = c"    
+    
+(* Left-cancellative semigroup *)
+class semigroup_add_left_cancel = semigroup_add + add_left_cancel
+  
 text \<open> In this algebra we only require zero_sum_right, but not
         zero_sum_left. The immediate consequence is that we do
-        not obtain an order as there is no anti-symmetry. \<close>
-    
-class fzero_sum_zero = fzero_add_zero +
-  assumes fzero_sum_right: "a + b = f0(b) \<Longrightarrow> b = f0(b)"
-    
-instance fzero_sum_zero \<subseteq> fzero_add_zero
-  by intro_classes  
-  
-instance fzero_add_zero \<subseteq> semigroup_add_fzero
-  by intro_classes
-    
-instance fzero_sum_zero \<subseteq> semigroup_add_fzero
-  by intro_classes    
-    
-text \<open> However, when in addition we consider the class fzero_is_0, then trivially we have that 
-       sum_left and sum properties are satisfied as expected. \<close>
-    
-lemma fzero_sum_left:
-  fixes a :: "'a::{fzero_is_0,fzero_sum_zero}"
-  shows "a + b = f0(a) \<Longrightarrow> a = f0(a)"
-  by (metis fzero_add_zero_class.add_fzero_right fzero_sum_right fzero_is_0)
-    
-lemma fzero_sum:
-  fixes a :: "'a::{fzero_is_0,fzero_sum_zero}"
-  shows "a + b = f0(a) \<longleftrightarrow> a = f0(a) \<and> b = f0(b)"
-  by (metis add_fzero_left fzero_is_0 fzero_sum_left)    
+        not obtain an order as there is no anti-symmetry. \<close>  
 
+(* USTA4 *)
+class fzero_sum_right = fzero + plus +
+  assumes fzero_sum_right: "a + b = f0(b) \<Longrightarrow> b = f0(b)"
+      
+(* USTA1+2 *)
+class fzero_add_zero = fzero_right_ident + semigroup_add_fzero
+begin
+  
 text \<open> We define less and minus in terms of plus in the context of the class fzero_add_zero
        as this is sufficient to define a prefix relation that is reflexive and transitive. \<close>
-
-context fzero_add_zero
-begin
   
 definition fzero_le (infix "\<le>us" 50)
   where "a \<le>us b \<longleftrightarrow> (\<exists>c. b = a + c)"
@@ -351,9 +330,6 @@ lemma fzero_le_trans:
   "\<lbrakk> a \<le>us b; b \<le>us c \<rbrakk> \<Longrightarrow> a \<le>us c"
   unfolding fzero_le_def
   using add_assoc by blast
-
-lemma fzero_le_least_fzero: "fzero a \<le>us a"
-  by (metis local.add_fzero_left local.fzero_le_def)
    
 lemma fzero_le_add: "a \<le>us a + b"
   using fzero_le_def
@@ -362,42 +338,51 @@ lemma fzero_le_add: "a \<le>us a + b"
 lemma fzero_le_add_left_mono: 
   "a \<le>us b \<Longrightarrow> c + a \<le>us c + b"
   using fzero_le_def
-  using add_assoc by auto
-
+  using add_assoc by auto  
+  
 end
-
-text \<open> The following class allows @term{\<le>}, @term{<} and @term{-} to be related with
-       that of fzero_add_zero. \<close>
-
-class fzero_add_fzero_ord = fzero_add_zero + ord + 
-  assumes le_is_fzero_le: "a \<le> b \<longleftrightarrow> (a \<le>us b)"
-  and less_iff: "a < b \<longleftrightarrow> a \<le> b \<and> \<not> (b \<le> a)"
-  
-class fzero_add_fzero_ord_minus = fzero_add_fzero_ord + ord + minus +
-  assumes minus_def: "a - b = a -us b"
-
-text \<open> We then show we have a preorder. \<close>
-
-instance fzero_add_fzero_ord \<subseteq> preorder
-proof
-  fix x y z :: "'a::fzero_add_fzero_ord" 
-  show "(x < y) = (x \<le> y \<and> \<not> y \<le> x)"
-    by (simp add: less_iff)
-  show "x \<le> x"
-    by (simp add: fzero_add_zero_class.fzero_refl le_is_fzero_le)
-  show "x \<le> y \<Longrightarrow> y \<le> z \<Longrightarrow> x \<le> z"
-    using le_is_fzero_le 
-    by (metis fzero_add_zero_class.fzero_le_trans)
-qed
-
-subsection \<open> Unary left-cancellative fzero semigroup class \<close>
-  
-class semigroup_add_left_cancel = semigroup_add +
-  assumes add_left_imp_eq: "a + b = a + c \<Longrightarrow> b = c"
-
-class fzero_add_left_cancel = semigroup_add_left_cancel + fzero_add_zero 
+    
+(* USTA1+2+3 *)
+class fzero_semigroup_left_cancel = add_left_cancel + fzero_add_zero 
 begin
   
+lemma add_fzero_left[simp]: "f0(a) + a = a"
+  by (metis add_assoc local.add_fzero_right local.add_left_imp_eq)
+  
+lemma fzero_idem[simp]: "f0(f0(a)) = f0(a)"
+  by (metis add_assoc local.add_fzero_right local.add_left_imp_eq)
+    
+(* This property is key for lifting the results on stlists. *)
+lemma add_fzero_any_left[simp]: "f0(b) + a = a"
+  by (metis add_assoc local.add_fzero_right local.add_left_imp_eq)
+    
+(* TODO: Add lemma1/2 here to aid readability of proofs. *)
+    
+lemma fzero_plus_left: "f0(y) = f0(x) + f0(y)"
+proof -
+  have "(x + y) + f0(x + y) = x + y"
+    by simp
+  then have "(x + y) + f0(x + y) = (x + y) + f0(y)"
+    by (simp add: add_assoc)
+  then have "f0(x + y) = f0(y)"
+    using local.add_left_imp_eq by blast
+  then show ?thesis by simp
+qed  
+    
+lemma fzero_plus_anihilate: "f0(x + y) = f0(y)"
+proof -
+  have "(x + y) + f0(x + y) = x + y"
+    by simp
+  then have "(x + y) + f0(x + y) = (x + y) + f0(y)"
+    by (simp add: add_assoc)
+  then have "f0(x + y) = f0(y)"
+    using local.add_left_imp_eq by blast
+  then show ?thesis by simp
+qed  
+  
+text \<open> A number of properties about concatenation and subtraction can be proved using
+       USTA1-3. \<close>
+    
 lemma add_fzero_diff_cancel_left [simp]: 
   "(a + b) -us a = b"
   apply (simp add: fzero_subtract_def fzero_le_add)
@@ -415,16 +400,89 @@ lemma diff_add_cancel_left': "a \<le>us b \<Longrightarrow> a + (b -us a) = b"
   by (metis add_fzero_diff_cancel_left local.fzero_le_def)
 
 lemma "b \<le>us a \<Longrightarrow> x = a -us b \<longleftrightarrow> b + x = a"
-  by (metis diff_add_cancel_left' local.add_left_imp_eq)
-
-end 
+  by (metis diff_add_cancel_left' local.add_left_imp_eq)  
   
-class fzero_add_zero_any_left_cancel = fzero_add_left_cancel + fzero_add_zero_any
+end
   
-class semigroup_add_left_cancel_minus_ord = fzero_add_fzero_ord_minus + fzero_add_left_cancel
+instance fzero_semigroup_left_cancel \<subseteq> semigroup_add_left_cancel
+  by intro_classes
+  
+(* USTA1+2+4 *)
+class fzero_sum_zero = fzero_add_zero + fzero_sum_right
+    
+(* USTA1+2+3+4 *)
+class usta_semigroup = fzero_sum_zero + fzero_semigroup_left_cancel
 begin
   
-  lemma le_iff_add: "a \<le> b \<longleftrightarrow> (\<exists> c. b = a + c)"
+text \<open> To show that every fzero is a least element, USTA4 is required in addition. \<close>
+  
+lemma fzero_le_least_fzero: "fzero a \<le>us b"
+  by (metis local.add.semigroup_axioms local.add_fzero_right local.add_left_imp_eq semigroup.assoc local.fzero_le_def)
+
+end
+  
+(* Axiom independence *)
+
+lemma 
+  fixes a :: "'a::fzero_semigroup_left_cancel" (* USTA1+2+3 *)
+  shows "a + b = f0(b) \<Longrightarrow> b = f0(b)" (* USTA4 *)
+  nitpick[expect=genuine] oops
+    
+lemma 
+  fixes a :: "'a::{fzero_add_zero,fzero_sum_right}" (* USTA1+2+4 *)
+  shows "a + b = a + c \<Longrightarrow> b = c" (* USTA3 *)
+  nitpick[expect=genuine] oops
+    
+lemma 
+  fixes a :: "'a::{semigroup_add_fzero,add_left_cancel,fzero_sum_right}" (* USTA1+3+4 *)
+  shows "a + f0(a) = a" (* USTA2 *)
+  nitpick[expect=genuine] oops
+    
+lemma 
+  fixes a :: "'a::{fzero_right_ident,add_left_cancel,fzero_sum_right}" (* USTA2+3+4 *)
+  shows "(a + b) + c = a + (b + c)" (* USTA1 *)
+  nitpick[expect=genuine] oops
+  
+(* defines operators in the context of usta_semigroup *)    
+    
+(* define usta_trace as usta_semigroup + ops + eqs mapping \<le> and \<le>\<^sub>u\<^sub>s *)    
+    
+(********* OLD BELOW *********)    
+    
+instance fzero_sum_zero \<subseteq> fzero_add_zero
+  by intro_classes  
+  
+instance fzero_add_zero \<subseteq> semigroup_add_fzero
+  by intro_classes
+    
+instance fzero_sum_zero \<subseteq> semigroup_add_fzero
+  by intro_classes    
+    
+text \<open> However, when in addition we consider the class fzero_is_0, then trivially we have that 
+       sum_left and sum properties are satisfied as expected. \<close>
+    
+lemma fzero_sum_left:
+  fixes a :: "'a::{fzero_is_0,fzero_sum_zero}"
+  shows "a + b = f0(a) \<Longrightarrow> a = f0(a)"
+  by (metis add_fzero_right fzero_is_0 fzero_sum_right) 
+                                        
+lemma fzero_sum:
+  fixes a :: "'a::{fzero_is_0,fzero_sum_zero}"
+  shows "a + b = f0(a) \<longleftrightarrow> a = f0(a) \<and> b = f0(b)"
+  by (metis add_fzero_right fzero_is_0 fzero_sum_right)
+
+
+  
+text \<open> A USTA semigroup whose @term{\<le>}, @term{<} and @term{-} are related with
+       the operators defined for a USTA.  \<close>  
+  
+class usta_trace = usta_semigroup + ord + minus +
+  assumes le_is_fzero_le: "a \<le> b \<longleftrightarrow> (a \<le>us b)"
+  and less_iff: "a < b \<longleftrightarrow> a \<le> b \<and> \<not> (b \<le> a)"
+  and minus_def: "a - b = a -us b"
+begin
+  
+lemma le_iff_add: "a \<le> b \<longleftrightarrow> (\<exists> c. b = a + c)"
     by (simp add: local.fzero_le_def local.le_is_fzero_le)
   
   lemma le_add [simp]: "a \<le> a + b"
@@ -507,17 +565,26 @@ begin
       
   (* SSub:subsub *)    
   lemma ssub_subsub: "c \<le> a \<and> c \<le> b \<and> b \<le> a \<longrightarrow>(a - c) - (b - c) = a - b"
-    by (metis local.diff_add_cancel_left' local.sum_minus_right)
-      
-end
-
-text \<open> Following the approach in Trace_Algebra we define a @{term pre_trace} class,
-       where in addition to satisfying @{term fzero_sum_zero}, and being a left cancellative
-       semigroup, also requires @{term sum_eq_sum_conv}. \<close>
+    by (metis local.diff_add_cancel_left' local.sum_minus_right)  
   
-class fzero_pre_trace = semigroup_add_left_cancel_minus_ord  +
-  assumes
-  sum_eq_sum_conv: "(a + b) = (c + d) \<Longrightarrow> \<exists> e . a = c + e \<and> e + b = d \<or> a + e = c \<and> b = e + d"
+end
+  
+instance usta_trace \<subseteq> preorder
+proof
+  fix x y z :: "'a::usta_trace" 
+  show "(x < y) = (x \<le> y \<and> \<not> y \<le> x)"
+    by (simp add: less_iff)
+  show "x \<le> x"
+    by (simp add: fzero_add_zero_class.fzero_refl le_is_fzero_le)
+  show "x \<le> y \<Longrightarrow> y \<le> z \<Longrightarrow> x \<le> z"
+    using le_is_fzero_le 
+    by (metis fzero_add_zero_class.fzero_le_trans)
+qed
+ 
+class sum_eq_sum_conv = plus +
+  assumes sum_eq_sum_conv: "(a + b) = (c + d) \<Longrightarrow> \<exists> e . a = c + e \<and> e + b = d \<or> a + e = c \<and> b = e + d"
+  
+class usta_trace_split = usta_trace + sum_eq_sum_conv
 begin
 
   text {* The set subtraces of a common trace $c$ is totally ordered *} 
@@ -536,17 +603,39 @@ begin
     
   lemma le_sum_iff: "a \<le> b + c \<longleftrightarrow> a \<le> b \<or> b \<le> a \<and> a - b \<le> c"
     by (metis local.add_le_imp_le_left local.add_left_mono local.diff_add_cancel_left' local.le_is_fzero_le local.le_sum_cases local.fzero_le_add local.fzero_le_trans)
-   
+  
+  text \<open> The following lemma requires fzero_sum_zero. \<close>
+  lemma neq_zero_impl_greater:
+    "x \<noteq> f0(x) \<Longrightarrow> f0(x) < x"
+    by (metis least_zero local.add_fzero_left local.diff_cancel local.fzero_sum_right local.less_iff sum_minus_left)    
 end
+  
+(** OLD BELOW **)
+  
+text \<open> The following class allows @term{\<le>}, @term{<} and @term{-} to be related with
+       that of fzero_add_zero. \<close>
 
-instance fzero_pre_trace \<subseteq> semigroup_add_fzero
-  by intro_classes  
+class fzero_add_fzero_ord = fzero_add_zero + ord + 
+  assumes le_is_fzero_le: "a \<le> b \<longleftrightarrow> (a \<le>us b)"
+  and less_iff: "a < b \<longleftrightarrow> a \<le> b \<and> \<not> (b \<le> a)"
+  
+class fzero_add_fzero_ord_minus = fzero_add_fzero_ord + ord + minus +
+  assumes minus_def: "a - b = a -us b"
+
+subsection \<open> Unary left-cancellative fzero semigroup class \<close>
+  
+text \<open> Following the approach in Trace_Algebra we define a @{term pre_trace} class,
+       where in addition to satisfying @{term fzero_sum_zero}, and being a left cancellative
+       semigroup, also requires @{term sum_eq_sum_conv}. \<close>
+
+instance usta_trace_split \<subseteq> semigroup_add_fzero
+  by intro_classes 
  
 text {* As stated earlier, there is no antisymmetry unless fzero
         is a constant. *}  
   
 lemma fzero_monoid_le_antisym :
-  fixes a :: "'a::{fzero_is_0,semigroup_add_left_cancel_minus_ord,fzero_sum_zero}"
+  fixes a :: "'a::{fzero_is_0,usta_trace_split}"
   assumes "a \<le>us b" "b \<le>us a"
   shows "a = b"
 proof -
@@ -557,7 +646,7 @@ proof -
     using assms(2) fzero_le_def by auto
 
   have "b' = (b' + a' + b')"
-    by (metis a' add.assoc b' semigroup_add_left_cancel_class.add_left_imp_eq)
+    by (metis a' add.assoc b' add_left_imp_eq)
     
   hence "f0(b') + f0(b') + b' = (b' + a' + b')"
     by (metis add.semigroup_axioms add_fzero_left semigroup.assoc)
@@ -578,84 +667,73 @@ proof -
 qed
 
 text \<open> We finally define the extended trace algebra that uses @{term f\<^sub>0}. \<close>
-
-class fzero_trace = fzero_pre_trace + semigroup_add_left_cancel_minus_ord + fzero_sum_zero
-begin
-  -- \<open> The following lemma requires fzero_sum_zero. \<close>
-  lemma neq_zero_impl_greater:
-    "x \<noteq> f0(x) \<Longrightarrow> f0(x) < x"
-    by (metis least_zero local.add_fzero_left local.diff_cancel local.fzero_sum_right local.less_iff sum_minus_left)
-end
   
 text {* This algebra forms a preorder. It turns out this is
         sufficient for the theories on reactive processes. *}  
-  
-instance fzero_trace \<subseteq> preorder
-  by (intro_classes)
  
 (* the following are properties satisfied by left/right restriction semigroups,
-   but the fzero_trace class does not satisfy all of them. I do not think that
+   but the usta_trace class does not satisfy all of them. I do not think that
    properties related to commutativity are ever satisfied in the general case. *)
     
 lemma fzero_restrict0:
-  fixes a :: "'a::fzero_trace"
+  fixes a :: "'a::usta_trace"
   shows "f0(f0(a) + b) = f0(a) + f0(b)"
   by (metis add.assoc add_fzero_diff_cancel_left add_fzero_right)
   
 lemma fzero_restrict1:
-  fixes a :: "'a::fzero_trace"
+  fixes a :: "'a::usta_trace"
   shows "f0(a) + b = b + f0(a + b)"
-  by (metis add.assoc add_fzero_right semigroup_add_left_cancel_class.add_left_imp_eq)
+  by (metis add.assoc add_fzero_right add_left_imp_eq)
   
 lemma fzero_dist_plus:
-  fixes a :: "'a::fzero_trace"
+  fixes a :: "'a::usta_trace"
   shows "f0(a + b) = f0(a) + f0(b)"
-  by (metis (no_types, lifting) fzero_idem fzero_restrict0 fzero_restrict1 semigroup_add_left_cancel_class.add_left_imp_eq)
+  by (metis (no_types, lifting) fzero_idem fzero_restrict0 fzero_restrict1 add_left_imp_eq)
  
 lemma 
-  fixes a :: "'a::fzero_trace"
+  fixes a :: "'a::usta_trace"
   shows "f0(a + b) = f0(b)"
-  by (metis add.assoc add_fzero_right semigroup_add_left_cancel_class.add_left_imp_eq)
+  by (metis add.assoc add_fzero_right add_left_imp_eq)
     
 lemma 
-  fixes x :: "'a::fzero_trace"
+  fixes x :: "'a::usta_trace"
   shows "(x + f0(x)) = x"
   by simp
     
 lemma    
-  fixes x :: "'a::fzero_trace"
-    and y :: "'a::fzero_trace"
+  fixes x :: "'a::usta_trace"
+    and y :: "'a::usta_trace"
   shows "f0(x + y) = f0(f0(x)+y)"
   by (simp add: fzero_dist_plus)
     
 lemma    
-  fixes x :: "'a::fzero_trace"
-    and y :: "'a::fzero_trace"
+  fixes x :: "'a::usta_trace"
+    and y :: "'a::usta_trace"
   shows "f0(f0(x) + f0(y)) = f0(y)+f0(x)+f0(y)"  
     by (metis (mono_tags, lifting) add.assoc fzero_dist_plus fzero_idem fzero_restrict1)
   
 lemma    
-  fixes x :: "'a::fzero_trace"
-    and y :: "'a::fzero_trace"
+  fixes x :: "'a::usta_trace"
+    and y :: "'a::usta_trace"
   shows "f0(x) + f0(x) = f0(x)"
   by (metis add_fzero_right fzero_idem)
     
-class fzero_is_0_sum_zero = fzero_is_0 + fzero_sum_zero
+class usta_semigroup_0 = fzero_is_0 + usta_semigroup
 
-instance fzero_is_0_sum_zero \<subseteq> monoid_sum_0
+instance usta_semigroup_0 \<subseteq> monoid_sum_0
   apply intro_classes
-  apply (metis add_fzero_left fzero_is_0)
-  apply (metis add_fzero_right fzero_is_0)
+    apply (metis add_fzero_left fzero_is_0)
+   apply (metis add_fzero_right fzero_is_0)
   by (metis fzero_is_0 fzero_sum)
 
 text \<open> A semigroup trace with a fixed zero (@{term fzero_is_0}) 
        is a monoid. \<close>
 
-class fzero_trace_0 = fzero_trace + fzero_is_0
+class usta_trace_0 = usta_trace + fzero_is_0
 
-instance fzero_trace_0 \<subseteq> monoid_add
+instance usta_trace_0 \<subseteq> monoid_add
 proof
-  fix a :: "'a::fzero_trace_0"
+  fix a :: "'a::usta_trace_0"
   show add_fzero_left: 
     "0 + a = a"
     by (metis add_fzero_right fzero_is_0 fzero_restrict1)
@@ -666,28 +744,33 @@ qed
 
 text \<open> A semigroup trace with a fixed zero (@{term fzero_is_0}) 
        is a monoid trace. \<close>
+  
+class usta_trace_split_0 = usta_trace_split + fzero_is_0
 
-instance fzero_trace_0 \<subseteq> trace 
+instance usta_trace_split_0 \<subseteq> usta_trace_0
+  by intro_classes
+  
+instance usta_trace_split_0 \<subseteq> trace 
 proof
-  fix a b c d :: "'a::fzero_trace_0"
-  show left_cancellative: 
+  fix a b c d :: "'a::usta_trace_split_0"
+  show left_cancellative:
     "a + b = a + c \<Longrightarrow> b = c"
-    using semigroup_add_left_cancel_class.add_left_imp_eq by blast
+    using add_left_imp_eq by blast
   show sum_left_zero:
     "a + b = 0 \<Longrightarrow> a = 0"
-    by (metis add.right_neutral add_fzero_right fzero_sum_left semigroup_add_left_cancel_class.add_left_imp_eq)
+    by (metis fzero_is_0 fzero_sum_left)
   show sum_eq_conv:
     "a + b = c + d \<Longrightarrow> \<exists>e. a = c + e \<and> e + b = d \<or> a + e = c \<and> b = e + d"
-    by (simp add: fzero_pre_trace_class.sum_eq_sum_conv)
+    by (simp add: sum_eq_sum_conv)
   show monoid_le:
     "(a \<le> b) = (a \<le>\<^sub>m b)"
-    by (simp add: monoid_le_def semigroup_add_left_cancel_minus_ord_class.le_iff_add)
+    by (simp add: monoid_le_def le_iff_add)
   show less:
     "(a < b) = (a \<le> b \<and> \<not> b \<le> a)"
-    by (simp add: fzero_add_fzero_ord_class.less_iff)
+    by (simp add: usta_trace_class.less_iff)
   show minus:
     "a - b = a -\<^sub>m b"
-    by (metis fzero_add_fzero_ord_minus_class.minus_def fzero_is_0 fzero_subtract_def le_is_fzero_le monoid_le_def monoid_subtract_def semigroup_add_left_cancel_minus_ord_class.le_iff_add)
+    by (metis fzero_is_0 fzero_subtract_def monoid_le_def monoid_subtract_def usta_trace_class.le_iff_add usta_trace_class.le_is_fzero_le usta_trace_class.minus_def)
 qed
 
 text \<open> Similarly, a trace which has a fixed @{term f\<^sub>0} is a semigroup satisfying the 
@@ -698,17 +781,13 @@ class trace_fzero_0 = trace + fzero_is_0
 instance trace_fzero_0 \<subseteq> fzero_add_zero
 proof
   fix a b :: "'a::trace_fzero_0"
-  show "f0(f0(a)) = f0(a)"
-    by (simp add: fzero_is_0)
-  show "f0(b) + a = a"
-    by (simp add: fzero_is_0)
   show "a + f0(a) = a"
     by (simp add: fzero_is_0)
 qed
 
-text \<open> Hence such a trace is also a semigroup trace. \<close>
+text \<open> Hence such a trace is also a usta trace. \<close>
 
-instance trace_fzero_0 \<subseteq> fzero_trace
+instance trace_fzero_0 \<subseteq> usta_trace
 proof
   fix a b c d :: "'a::trace_fzero_0"
   show "(a \<le> b) = (a \<le>us b)"
@@ -719,41 +798,31 @@ proof
     by (metis fzero_is_0 fzero_le_def fzero_subtract_def le_is_monoid_le monoid_subtract_def trace_class.le_iff_add trace_class.minus_def)
   show "a + b = a + c \<Longrightarrow> b = c"
     by (metis left_cancel_semigroup_class.add_left_imp_eq)
-  show "a + b = c + d \<Longrightarrow> \<exists>e. a = c + e \<and> e + b = d \<or> a + e = c \<and> b = e + d"
-    by (simp add: pre_trace_class.sum_eq_sum_conv)
+  (**)
   show "a + b = f0(b) \<Longrightarrow> b = f0(b)"
     by (simp add: fzero_is_0 zero_sum_right)
 qed
-
+  
+instance trace_fzero_0 \<subseteq> usta_trace_split
+proof
+  fix a b c d :: "'a::trace_fzero_0"
+  show "a + b = c + d \<Longrightarrow> \<exists>e. a = c + e \<and> e + b = d \<or> a + e = c \<and> b = e + d"
+    by (simp add: pre_trace_class.sum_eq_sum_conv)
+qed
+  
 text \<open> Therefore, a semigroup trace with a fixed @{term f\<^sub>0} is exactly the same as the
        monoid trace. This is convenient as any type instantiated with the class @{class trace}
-       can also be instantiated with the class @{class fzero_trace} by defining an appropriate
+       can also be instantiated with the class @{class usta_trace} by defining an appropriate
        @{term f\<^sub>0}. \<close>
-  
-  
-class fzero_add_any_pre_trace = fzero_add_zero_any_left_cancel + fzero_pre_trace  
-  
-class fzero_add_any_trace = fzero_add_zero_any + fzero_trace   
-  
-instance fzero_add_any_trace \<subseteq> fzero_add_any_pre_trace
-  by intro_classes  
-    
-instance trace_fzero_0 \<subseteq> fzero_add_zero_any
-  apply intro_classes
-  by (simp add: fzero_is_0)
-    
+      
 class fzero_add_zero_0 = fzero_add_zero + fzero_is_0
                
 class fzero_sum_zero_0 = fzero_sum_zero + fzero_is_0
   
 class fzero_almost_pre_trace_0 = left_cancel_semigroup + fzero_sum_zero + fzero_is_0  
-  
-class fzero_pre_trace_0 = fzero_pre_trace + fzero_is_0 + fzero_sum_zero(*left_cancel_semigroup + fzero_sum_zero_0*) 
- 
-instance fzero_add_zero_0 \<subseteq> monoid_add
-  apply intro_classes
-  using fzero_is_0 apply (metis add_fzero_left)
-  using fzero_is_0 by (metis add_fzero_right)
+   
+instance usta_trace_split_0 \<subseteq> monoid_add
+  by intro_classes
     
 instance fzero_almost_pre_trace_0 \<subseteq> left_cancel_semigroup
   by intro_classes
@@ -761,27 +830,20 @@ instance fzero_almost_pre_trace_0 \<subseteq> left_cancel_semigroup
 instance fzero_almost_pre_trace_0 \<subseteq> fzero_sum_zero_0
   by intro_classes
   
-instance fzero_sum_zero_0 \<subseteq> monoid_sum_0
-  apply intro_classes
-  using fzero_is_0 apply (metis add_fzero_left)
-  using fzero_is_0 apply (metis add_fzero_right)
-  using fzero_is_0 by (metis fzero_sum)
-
 instance semigroup_add_left_cancel \<subseteq> left_cancel_semigroup
   apply intro_classes
   by (simp add:add_left_imp_eq)    
     
-instance fzero_pre_trace_0 \<subseteq> fzero_sum_zero_0
+instance usta_trace_split_0 \<subseteq> fzero_sum_zero_0
   by intro_classes
 
-instance fzero_pre_trace_0 \<subseteq> pre_trace
-  apply intro_classes
-  using fzero_is_0 by (simp add: fzero_pre_trace_class.sum_eq_sum_conv)
+instance usta_trace_split_0 \<subseteq> pre_trace
+  by intro_classes
       
-instance fzero_trace_0 \<subseteq> fzero_trace
+instance usta_trace_0 \<subseteq> usta_trace
   by intro_classes
     
-instance fzero_pre_trace_0 \<subseteq> fzero_pre_trace
+instance usta_trace_split_0 \<subseteq> usta_trace_split
   by intro_classes
     
 section \<open> Models \<close>
@@ -849,7 +911,7 @@ lemma fzero_subtract_nat:
 instance nat :: trace_fzero_0
   by intro_classes
 
-instance nat :: fzero_trace
+instance nat :: usta_trace
   by intro_classes
   
 end
